<?xml version="1.0"?>
<rdf:RDF xmlns="http://www.semanticweb.org/robertomonaco/ontologies/2021/5/Energy_Framework#"
    xml:base="http://www.semanticweb.org/robertomonaco/ontologies/2021/5/Energy_Framework"
    xmlns:owl="http://www.w3.org/2002/07/owl#"
    xmlns:rdf="http://www.w3.org/1999/02/22-rdf-syntax-ns#"
    xmlns:xml="http://www.w3.org/XML/1998/namespace"
    xmlns:xsd="http://www.w3.org/2001/XMLSchema#"
    xmlns:rdfs="http://www.w3.org/2000/01/rdf-schema#">


    <owl:Class
        rdf:about="http://www.semanticweb.org/robertomonaco/ontologies/2021/5/Energy_Framework#Thing">
        <rdfs:label xml:lang="en">Thing</rdfs:label>
        <rdfs:comment xml:lang="en">The root class of the ontology, representing any object or
            concept.</rdfs:comment>
    </owl:Class>

    <owl:Class
        rdf:about="http://www.semanticweb.org/robertomonaco/ontologies/2021/5/Energy_Framework#Markets">
        <rdfs:subClassOf rdf:resource="http://www.w3.org/2002/07/owl#Thing" />
        <rdfs:comment xml:lang="en">Market designs impacts on how to determine the market clearing
            price.
            Each design will result in different energy dispatch and market price per agent.
            It sometimes also refers to the roles and responsibilities of different market actors
            and the processes between them. This involves among other questions on what market model
            is used, who the players are, how they interact, what tariff structure is in place and
            whether additional constraints such as taxes or subsidy schemes may apply.</rdfs:comment>
    </owl:Class>

    <owl:Class
        rdf:about="http://www.semanticweb.org/robertomonaco/ontologies/2021/5/Energy_Framework#Electricity_market">
        <rdfs:subClassOf
            rdf:resource="http://www.semanticweb.org/robertomonaco/ontologies/2021/5/Energy_Framework#Markets" />
        <rdfs:comment xml:lang="en">Market relating to the supply and use of electricity as a form
            of energy</rdfs:comment>
    </owl:Class>


    <owl:Class
        rdf:about="http://www.semanticweb.org/robertomonaco/ontologies/2021/5/Energy_Framework#MarketActor">
        <rdfs:subClassOf rdf:resource="http://www.w3.org/2002/07/owl#Thing" />
        <rdfs:comment xml:lang="en">A market actor is a participant in an energy market, such as a
            utility company, generator, or consumer.</rdfs:comment>
    </owl:Class>

    <owl:Class
        rdf:about="http://www.semanticweb.org/robertomonaco/ontologies/2021/5/Energy_Framework#Agent">
        <rdfs:subClassOf rdf:resource="http://www.w3.org/2002/07/owl#Thing" />
        <rdfs:comment xml:lang="en">An agent is a general term used to refer to any entity that can
            act or make decisions, such as a person, organization, or software program.</rdfs:comment>
    </owl:Class>


    <owl:ObjectProperty
        rdf:about="http://www.semanticweb.org/robertomonaco/ontologies/2021/5/Energy_Framework#hasMarketActor">
        <rdfs:domain
            rdf:resource="http://www.semanticweb.org/robertomonaco/ontologies/2021/5/Energy_Framework#Markets" />
        <rdfs:range
            rdf:resource="http://www.semanticweb.org/robertomonaco/ontologies/2021/5/Energy_Framework#MarketActor" />
        <rdfs:comment xml:lang="en">Property to link a market to its market actors</rdfs:comment>
    </owl:ObjectProperty>

    <owl:DatatypeProperty
        rdf:about="http://www.semanticweb.org/robertomonaco/ontologies/2021/5/Energy_Framework#marketType">
        <rdfs:domain
            rdf:resource="http://www.semanticweb.org/robertomonaco/ontologies/2021/5/Energy_Framework#Markets" />
        <rdfs:range rdf:resource="http://www.w3.org/2001/XMLSchema#string" />
        <rdfs:label xml:lang="en">marketType</rdfs:label>
        <rdfs:comment xml:lang="en">The type of the market, such as an electricity or gas market.</rdfs:comment>
    </owl:DatatypeProperty>

    <owl:DatatypeProperty
        rdf:about="http://www.semanticweb.org/robertomonaco/ontologies/2021/5/Energy_Framework#marketClearingPrice">
        <rdfs:domain
            rdf:resource="http://www.semanticweb.org/robertomonaco/ontologies/2021/5/Energy_Framework#Markets" />
        <rdfs:range rdf:resource="http://www.w3.org/2001/XMLSchema#float" />
        <rdfs:label xml:lang="en">marketClearingPrice</rdfs:label>
        <rdfs:comment xml:lang="en">The market clearing price for the market.</rdfs:comment>
    </owl:DatatypeProperty>


    <owl:DatatypeProperty
        rdf:about="http://www.semanticweb.org/robertomonaco/ontologies/2021/5/Energy_Framework#agentName">
        <rdfs:domain
            rdf:resource="http://www.semanticweb.org/robertomonaco/ontologies/2021/5/Energy_Framework#Agent" />
        <rdfs:range rdf:resource="http://www.w3.org/2001/XMLSchema#string" />
        <rdfs:label xml:lang="en">agentName</rdfs:label>
        <rdfs:comment xml:lang="en">The name of the agent.</rdfs:comment>
    </owl:DatatypeProperty>

    <owl:DatatypeProperty
        rdf:about="http://www.semanticweb.org/robertomonaco/ontologies/2021/5/Energy_Framework#agentType">
        <rdfs:domain
            rdf:resource="http://www.semanticweb.org/robertomonaco/ontologies/2021/5/Energy_Framework#Agent" />
        <rdfs:range rdf:resource="http://www.w3.org/2001/XMLSchema#string" />
        <rdfs:label xml:lang="en">agentType</rdfs:label>
        <rdfs:comment xml:lang="en">The type of agent, such as a producer or consumer.</rdfs:comment>
    </owl:DatatypeProperty>

    <owl:DatatypeProperty
        rdf:about="http://www.semanticweb.org/robertomonaco/ontologies/2021/5/Energy_Framework#agentMarketParticipation">
        <rdfs:domain
            rdf:resource="http://www.semanticweb.org/robertomonaco/ontologies/2021/5/Energy_Framework#Agent" />
        <rdfs:range rdf:resource="http://www.w3.org/2001/XMLSchema#string" />
        <rdfs:label xml:lang="en">agentMarketParticipation</rdfs:label>
        <rdfs:comment xml:lang="en">The market in which the agent is participating, such as the
            electricity or gas market.</rdfs:comment>
    </owl:DatatypeProperty>


    <owl:DatatypeProperty
        rdf:about="http://www.semanticweb.org/robertomonaco/ontologies/2021/5/Energy_Framework#marketActorId">
        <rdfs:domain
            rdf:resource="http://www.semanticweb.org/robertomonaco/ontologies/2021/5/Energy_Framework#MarketActor" />
        <rdfs:range rdf:resource="http://www.w3.org/2001/XMLSchema#string" />
        <rdfs:label xml:lang="en">marketActorId</rdfs:label>
        <rdfs:comment xml:lang="en">The unique identifier of the market actor.</rdfs:comment>
    </owl:DatatypeProperty>

    <owl:DatatypeProperty
        rdf:about="http://www.semanticweb.org/robertomonaco/ontologies/2021/5/Energy_Framework#marketActorRole">
        <rdfs:domain
            rdf:resource="http://www.semanticweb.org/robertomonaco/ontologies/2021/5/Energy_Framework#MarketActor" />
        <rdfs:range rdf:resource="http://www.w3.org/2001/XMLSchema#string" />
        <rdfs:label xml:lang="en">marketActorRole</rdfs:label>
        <rdfs:comment xml:lang="en">The role of the market actor, such as generator or distributor.</rdfs:comment>
    </owl:DatatypeProperty>

    <owl:DatatypeProperty
        rdf:about="http://www.semanticweb.org/robertomonaco/ontologies/2021/5/Energy_Framework#marketActorCompany">
        <rdfs:domain
            rdf:resource="http://www.semanticweb.org/robertomonaco/ontologies/2021/5/Energy_Framework#MarketActor" />
        <rdfs:range rdf:resource="http://www.w3.org/2001/XMLSchema#string" />
        <rdfs:label xml:lang="en">marketActorCompany</rdfs:label>
        <rdfs:comment xml:lang="en">The company which the market actor belongs to.</rdfs:comment>
    </owl:DatatypeProperty>


    <owl:DatatypeProperty
        rdf:about="http://www.semanticweb.org/robertomonaco/ontologies/2021/5/Energy_Framework#marketDesign">
        <rdfs:domain
            rdf:resource="http://www.semanticweb.org/robertomonaco/ontologies/2021/5/Energy_Framework#Electricity_market" />
        <rdfs:range rdf:resource="http://www.w3.org/2001/XMLSchema#string" />
        <rdfs:label xml:lang="en">marketDesign</rdfs:label>
        <rdfs:comment xml:lang="en">The design of the electricity market, such as spot market or
            auction market.</rdfs:comment>
    </owl:DatatypeProperty>

    <owl:DatatypeProperty
        rdf:about="http://www.semanticweb.org/robertomonaco/ontologies/2021/5/Energy_Framework#marketRegulation">
        <rdfs:domain
            rdf:resource="http://www.semanticweb.org/robertomonaco/ontologies/2021/5/Energy_Framework#Electricity_market" />
        <rdfs:range rdf:resource="http://www.w3.org/2001/XMLSchema#string" />
        <rdfs:label xml:lang="en">marketRegulation</rdfs:label>
        <rdfs:comment xml:lang="en">The regulation of the electricity market, such as deregulated or
            regulated market.</rdfs:comment>
    </owl:DatatypeProperty>
</rdf:RDF>